some of the refinement laws are done

InsertionSort.dfy
@@ -1,19 +1,88 @@
 
 method PairInsertionSort(a: array<int>)
-	requires a.Length>1
 	ensures Sorted1(a,0,a.Length-1)
 	ensures multiset(a[..]) == multiset(old(a[..]))
 	modifies a
 {
-	ghost var A := multiset(a[..]);
-	var i,j,x,y;
-	i:=0;
-	j:=i-1;
-	while i < a.Length-1
-		decreases a.Length - i
-		invariant InvPair(a[..],i,j,A)
+	//introdue local variable + leading assignemnt + weaken precondition
+	ghost var A := multiset(old(a[..]));
+	PairInsertionSort1(a,A);
+}
+method PairInsertionSort1(a: array<int>, ghost A: multiset<int>) 	
+	requires multiset(a[..])==A
+	ensures Sorted1(a,0,a.Length-1)
+	ensures multiset(a[..]) == A
+	modifies a
+{
+	//introduce local variables+sequential composition
+	var i:nat;
+	var j,x,y;
+	j,i:=initIJ(a,j,i,A);
+	j,i,x,y:=PairInsertionSort2(a,j,i,x,y,A);
+}
+method initIJ(ghost a: array<int>, j0: int,i0:nat, ghost A: multiset<int>) returns (j: int,i:nat)
+	requires multiset(a[..])==A
+	ensures InvPair(a[..],j,i,A)
+	modifies a
 	{
-		x,y:=a[i],a[i+1];
+		//assignment
+		LemmainitIJ(a,j,i,A);
+		j,i:=j0,i0;
+		j,i:=-1,0;
+	}
+lemma LemmainitIJ( a: array<int>, j: int,i:nat,  A: multiset<int>)
+	requires multiset(a[..])==A
+	ensures InvPair(a[..],-1,0,A)
+{}
+
+method PairInsertionSort2(a: array<int>, j0: int,i0:nat,x0:int, y0:int, ghost A: multiset<int>) returns (j: int,i:nat,x:int,y:int)
+	requires InvPair(a[..],j0,i0,A)
+	ensures Sorted1(a,0,a.Length-1)
+	ensures multiset(a[..]) == A
+	modifies a
+{
+	//sequential composition
+	j,i,x,y:=j0,i0,x0,y0;
+	j,i,x,y:=MainLoop(a,j,i,x,y,A);
+	if i==a.Length-1{
+		j,y := i-1,a[i];
+		while j>=0 && a[j] >y
+			invariant Inv4Pair(a[..],j,i,x,y,A)
+			decreases j
+		{
+			SwapPair(a,j+1,j,A);
+			j:=j-1;
+		}
+	}
+	else {
+
+	}	
+
+}
+
+method MainLoop(a: array<int>, j0: int,i0:nat,x0:int, y0:int, ghost A: multiset<int>) returns (j: int,i:nat,x:int,y:int)
+	requires InvPair(a[..],j0,i0,A)
+	ensures InvPair(a[..],j,i,A) && !GuardMainLoop(a,i)
+	modifies a
+
+{
+	//iteration
+	j,i,x,y:=j0,i0,x0,y0;
+	while GuardMainLoop(a,i)
+		decreases a.Length - i
+		invariant InvPair(a[..],j,i,A)
+	{
+		j,i,x,y:=MainLoopBody(a,j,i,x,y,A);
+	}
+}
+
+method MainLoopBody(a: array<int>, j0: int,i0:nat,x0:int, y0:int, ghost A: multiset<int>) returns (j: int,i:nat,x:int,y:int)
+	requires InvPair(a[..],j0,i0,A) && GuardMainLoop(a,i0)
+	ensures InvPair(a[..],j,i,A) && (a.Length-i)< (a.Length-i0)
+	modifies a
+{
+	j,i,x,y:=j0,i0,x0,y0;
+	x,y:=a[i],a[i+1];
 		if x<y {
 			x,y:=y,x;
 		}
@@ -46,25 +115,18 @@ method PairInsertionSort(a: array<int>)
 			}
 		
 		i:=i+2;	
-	}
-
-	if i==a.Length-1{
-		j,y := i-1,a[i];
-		while j>=0 && a[j] >y
-			invariant Inv4Pair(a[..],j,i,x,y,A)
-			decreases j
-		{
-			SwapPair(a,j+1,j,A);
-			j:=j-1;
-		}
-	}
-	else {
-
-	}	
-
 }
-
-
+predicate method GuardMainLoop(a: array<int>,i:nat)
+{
+	i < a.Length-1	
+}
+predicate InvPair(a: seq<int>, j: int, i:nat, A: multiset<int>)
+{
+	0<=i<=|a| &&
+	(|a|>1 ==> (-1<=j<=|a|-3)) &&
+	SortedSequence1(a,0,i-1) &&
+	multiset(a)==A
+}
 predicate Inv2Pair(a: seq<int>, j: int,i:nat,x:int, y:int, A: multiset<int>)
 {
 	0<=i<=|a|-2 &&
@@ -77,25 +139,7 @@ predicate Inv2Pair(a: seq<int>, j: int,i:nat,x:int, y:int, A: multiset<int>)
 	multiset(a)==A
 }
 
-predicate Sorted1(a: array<int>, i:nat, j:int)
-	requires i<=j ==> (0<=i<a.Length && 0<=j<a.Length)
-	reads a
-{
-	 (forall k :: i <= k < j-1 ==> a[k] <= a[k+1]) 
-}
-predicate InvPair(a: seq<int>, i: nat, j:int, A: multiset<int>)
-{
-	0<=i<=|a| &&
-	(-1<=j<=|a|-3) &&
-	SortedSequence1(a,0,i-1) &&
-	multiset(a)==A
-}
 
-predicate SortedSequence1(a: seq<int>, i:nat, h:int)
-	requires i<=h ==> (0<=i <|a| && 0<=h<|a|)
-{
-	(forall k :: i <=  k <= h-1 ==> a[k] <= a[k+1])
-}
 
 lemma LemmaMidswap(a: seq<int>,j:int,i:nat,x:int,y:int, A: multiset<int>)
 	requires Inv2Pair(a,j,i,x,y,A)
@@ -153,7 +197,21 @@ predicate Inv4Pair(a: seq<int>, j: int,i:nat,x:int, y:int, A: multiset<int>)
 
 
 
+predicate Sorted1(a: array<int>, i:nat, j:int)
+	requires i<=j ==> (0<=i<a.Length && 0<=j<a.Length)
+	reads a
+{
+	 (forall k :: i <= k < j-1 ==> a[k] <= a[k+1]) 
+}
 
+
+
+
+predicate SortedSequence1(a: seq<int>, i:nat, h:int)
+	requires i<=h ==> (0<=i <|a| && 0<=h<|a|)
+{
+	(forall k :: i <=  k <= h-1 ==> a[k] <= a[k+1])
+}
 
 method {:verify true} SwapPair(a: array<int>, x:nat,y:nat,ghost A: multiset<int>)
 	requires multiset(a[..]) == A
